removed old files

fairis/heap_lang/examples/even_odd/eo_vs_mod.v
@@ -9,111 +9,22 @@ From trillium.program_logic Require Export weakestpre.
 From trillium.fairness Require Import fairness fair_termination.
 From trillium.fairness.heap_lang Require Export lang lifting tactics proofmode.
 From trillium.fairness.heap_lang Require Import notation.
-From trillium.fairness.heap_lang.examples.even_odd Require Import action_model.
-
-
-  Lemma ex_and_comm {T: Type} (A: Prop) (B: T -> Prop):
-    (exists t, A /\ B t) <-> A /\ exists t, B t.
-  Proof. split; intros (?&?&?); eauto. Qed.
-
+From trillium.fairness.heap_lang.examples.even_odd Require Import action_model interface utils thread_progs.
 Import derived_laws_later.bi.
 
 Open Scope nat.
 
 Set Default Proof Using "Type".
 
-Definition incr_loop : val :=
-  rec: "incr_loop" "l" "n" :=
-    (if: CAS "l" "n" ("n"+#1)
-     then "incr_loop" "l" ("n" + #2)
-     else "incr_loop" "l" "n").
-
-Definition start : val :=
-  λ: "l",
-    let: "x" := !"l" in
-    (Fork (incr_loop "l" "x") ;;
-    Fork (incr_loop "l" ("x"+#1))).
-
 
 Section Models.
+  Context {even_impl: EvenModel}.
+  Context {odd_impl: OddModel}.
 
-  Inductive PubA := step_sync (k: nat).
+  Let even_AM := @even_AM even_impl. 
+  Let odd_AM := @odd_AM odd_impl. 
 
-  Global Instance PubA_EqDec: EqDecision PubA.
-  Proof.
-    intros [x] [y]. destruct (decide (x = y)); [left | right]; set_solver.
-  Qed. 
-
-  Section ThreadModel.
-    Context (d: nat).
-
-    Definition PrivA := unit.
-    Let step_loop: PrivA := (). 
-    
-    Definition TA: Type := PubA + PrivA. 
-    Definition TR := unit.
-    Definition ρT: TR := (). 
-    
-    Definition TS := nat. 
-    
-    Inductive thread_trans: TS -> TA * option TR -> TS -> Prop :=
-    | thread_step n : Nat.even (n + d) → thread_trans n (inl (step_sync n), Some ρT) (S n)
-    | thread_loop n : Nat.odd (n + d) → thread_trans n (inr step_loop, Some ρT) n
-    | thread_env n : Nat.odd (n + d) → thread_trans n (inl (step_sync n), None) (S n)
-    .
-    
-    Definition thread_model: ActionModel := {| amTrans := thread_trans |}.
-
-    (* Global Instance TR_eqdec: EqDecision TR. *)
-    (* apply _.  *)
-    (* Qed.  *)
-
-    Lemma thread_AM_fin_branch': AM_fin_branch' thread_model.
-    Proof.
-      red. exists (fun n => n' ← [n; S n]; 
-                      a ← [inl $ step_sync n; inr step_loop];
-                      ρ ← [Some ρT; None]; mret (n', a, ρ)).
-      intros * STEP.
-      repeat (setoid_rewrite elem_of_list_bind).
-      setoid_rewrite elem_of_list_ret.
-      eexists. apply and_comm. rewrite -ex_and_comm.
-      eexists. apply and_comm. rewrite -!and_assoc. apply and_comm. rewrite -ex_and_comm.
-      eexists. apply and_comm. rewrite -!and_assoc.
-      split; [reflexivity| ].
-      inversion STEP; subst; set_solver.
-    Qed.
-
-    Lemma thread_AM_step_dec: AM_step_dec thread_model.
-    Proof.
-      red. intros.
-      Local Ltac contra := right; intros TRANS; inversion TRANS; subst; try tauto; try lia.
-      destruct (decide (Nat.even (s1 + d))).
-      - destruct (decide (s2 = S s1 /\ oρ = Some ρT /\ a = inl (step_sync s1))) as [(-> & -> & ->)|?].
-        + left. by econstructor.
-        + contra; rewrite -Nat.negb_even in H3; by apply negb_prop_elim in H3.
-      - pose proof n as n'. 
-        apply negb_prop_intro in n. rewrite Nat.negb_even in n.
-        destruct (decide (s2 = s1 /\ oρ = Some ρT /\ a = inr step_loop)) as [(-> & -> & ->)|?].
-        + left. by econstructor.
-        + destruct (decide (s2 = S s1 /\ oρ = None /\ a = inl (step_sync s1))) as [(-> & -> & ->)|?].
-          * left. by econstructor.
-          * contra.
-    Qed.
-
-    Lemma thread_AM_strong: AM_strong_lr thread_model.
-    Proof. 
-      apply fin_branch_strong; auto using thread_AM_step_dec, thread_AM_fin_branch'.
-    Qed.
-    
-    (* Opaque PrivA.  *)
-    (* Opaque TR.  *)
-      
-  End ThreadModel.
-  
-  Definition even_AM := thread_model 0. 
-  Definition odd_AM := thread_model 1.
-
-  Definition prodA: Type := PubA + (PrivA + PrivA). 
+  Definition prodA: Type := PubA + (@ePriv even_impl + @oPriv odd_impl). 
   Definition fact_TA (pa: prodA): option (amA even_AM) * option (amA odd_AM) := 
     match pa with
     | inl s => (Some $ inl s, Some $ inl s)
@@ -121,12 +32,16 @@ Section Models.
     | inr (inr p) => (None, Some $ inr p)
     end. 
 
-  Definition prod_model := ProdAM (fact_act := fact_TA). 
+  Definition prod_model := ProdAM (fact_act := fact_TA).
+
+  Existing Instance even_AME. 
+  Existing Instance odd_AME.
 
   Lemma prod_AM_fin_branch': AM_fin_branch' prod_model.
   Proof. 
-    unshelve eapply prod_AM_fin_branch'.  
-    2, 3: apply thread_AM_fin_branch'. 
+    unshelve eapply prod_AM_fin_branch'.
+    3: apply odd_AME. 
+    2: apply even_AME. 
     { exact (fun '(oa1, oa2) => 
                match oa1, oa2 with
                | Some (inl pa1), Some _ => inl pa1
@@ -135,46 +50,22 @@ Section Models.
                | _, _ => inl (step_sync 0)
                end). }
     red. intros [?|[?|?]]; reflexivity.
-  Qed. 
+  Qed.
 
   Lemma prod_AM_strong_lr: AM_strong_lr prod_model.
   Proof. 
     apply fin_branch_strong.
     - apply prod_AM_fin_branch'. 
-    - apply prod_AM_step_dec; apply thread_AM_step_dec.
+    - unshelve eapply prod_AM_step_dec.
+      + apply even_AME.
+      + apply odd_AME. 
   Qed.
 
   Definition the_fair_model: FairModel.
     unshelve eapply (AM2FM prod_model). 
-  Proof.
+  Proof using even_impl odd_impl.
     apply prod_AM_strong_lr. 
   Defined.
-
-  Lemma tfm_live_roles st: 
-    live_roles the_fair_model st =
-     set_map inl (AM_live_roles (thread_AM_strong 0) st.1) ∪
-     set_map inr (AM_live_roles (thread_AM_strong 1) st.2).
-  Proof.
-    destruct st as [st1 st2]. simpl.
-    apply set_eq. intros ρ.
-    rewrite elem_of_union. rewrite !elem_of_map. 
-    setoid_rewrite <- (AM_live_roles_spec prod_AM_strong_lr).
-    setoid_rewrite <- (AM_live_roles_spec (thread_AM_strong 0)).
-    setoid_rewrite <- (AM_live_roles_spec (thread_AM_strong 1)).
-    split.
-    - intros (?&?&STEP). inversion STEP; subst.
-      1, 3: by left; eexists; split; eauto. 
-      all: by right; eexists; split; eauto.
-    - (* !!! relies on the definition of thread_model *)
-      (* !!! only holds in s1 = s2 *)
-      intros [[ρ1 [-> (a1&?&STEP)]]| [? [-> (?&?&STEP)]]].
-      + simpl in a1. unfold TA in a1.
-        destruct a1 as [[n]| ].
-        * inversion STEP; subst. rewrite Nat.add_0_r in H3.
-          eexists _, (_, _). simpl.
-          eapply (@pt_sync1 _ _ _ fact_TA); eauto.
-          2: { eapply thread_env.        
-  Abort. 
 
   Definition the_model: LiveModel heap_lang the_fair_model :=
     {| lm_fl (x: fmstate the_fair_model) := 61%nat; |}.
@@ -182,277 +73,304 @@ Section Models.
 End Models.  
 
 (** The CMRAs we need. *)
-Class evenoddG Σ := EvenoddG {
+Class evenoddPreG (Σ: gFunctors) := {
+}.
+
+Class evenoddG (Σ: gFunctors) := EvenoddG {
   even_name: gname;
   odd_name: gname;
-  evenodd_n_G :> inG Σ (excl_authR natO);
+  eoPreG :> evenoddPreG Σ;
  }.
-Class evenoddPreG Σ := {
-  evenodd_PreG :> inG Σ (excl_authR natO);
- }.
-
-(* Definition evenoddΣ : gFunctors := *)
-(*   #[ heapΣ the_fair_model; GFunctor (excl_authR natO) ; GFunctor (excl_authR boolO) ]. *)
-
-(* Global Instance subG_evenoddΣ {Σ} : subG evenoddΣ Σ → evenoddPreG Σ. *)
-(* Proof. solve_inG. Qed. *)
 
 Section proof.
-  Context `{!heapGS Σ the_model, !evenoddG Σ}.
-  (* Context `{EM__G: ExecutionModel heap_lang M__G} `{@heapGS Σ _ EM__G, evenoddG Σ}. *)
-  (* Context {ifG: fairnessGS the_model Σ}. *)
+  Context {even_impl: EvenModel} {odd_impl: OddModel}.
+
+  Let M := @the_fair_model even_impl odd_impl.
+  Let LM := @the_model even_impl odd_impl.
+  Context `{!heapGS Σ LM, !evenoddG Σ}.
+  Context {th_preG: threadPreG Σ}. 
+
+  Existing Instance even_AME. 
+  Existing Instance odd_AME.
 
   Let Ns := nroot .@ "even_odd".
 
-  Definition even_at (n: nat) := own even_name (◯E n).
-  Definition odd_at (n: nat) := own odd_name (◯E n).
+  Local Instance evenThreadG: threadG Σ := {| th_name := even_name |}. 
+  Local Instance oddThreadG: threadG Σ := {| th_name := odd_name |}. 
 
-  Definition auth_even_at (n: nat) := own even_name (●E n).
-  Definition auth_odd_at (n: nat) := own odd_name (●E n).
+  Definition even_at := (@th_at _ evenThreadG). 
+  Definition odd_at := (@th_at _ oddThreadG). 
 
-  Lemma they_agree γ (N M: nat) :
-    own γ (◯E N) -∗ own γ (●E M) -∗ ⌜ M = N ⌝.
-  Proof.
-    iIntros "HA HB". iCombine "HB HA" as "H".
-    iDestruct (own_valid with "H") as "%Hval".
-    iPureIntro. by apply excl_auth_agree_L.
-  Qed.
-  Lemma even_agree N M :
-    even_at N -∗ auth_even_at M -∗ ⌜ M = N ⌝.
-  Proof. apply they_agree. Qed.
-  Lemma odd_agree N M :
-    odd_at N -∗ auth_odd_at M -∗ ⌜ M = N ⌝.
-  Proof. apply they_agree. Qed.
+  Definition auth_even_at := (@auth_th_at _ evenThreadG). 
+  Definition auth_odd_at := (@auth_th_at _ oddThreadG).  
 
-  Lemma they_update γ (N M P: nat) :
-    own γ (●E N) ∗ own γ (◯E M) ==∗ own γ (●E P) ∗ own γ (◯E P).
-  Proof.
-    rewrite -!own_op. iApply own_update. apply excl_auth_update.
-  Qed.
-  Lemma even_update P N M:
-     auth_even_at M ∗ even_at N ==∗ auth_even_at P ∗ even_at P.
-  Proof. apply they_update. Qed.
-  Lemma odd_update P N M:
-     auth_odd_at M ∗ odd_at N ==∗ auth_odd_at P ∗ odd_at P.
-  Proof. apply they_update. Qed.
-
-  Definition evenodd_inv_inner n : iProp Σ :=
-    ∃ N,
-      frag_model_is (N, N) ∗ n ↦ #N ∗
+  Definition evenodd_inv_inner l : iProp Σ :=
+    ∃ st__e st__o N,
+      frag_model_is (st__e, st__o) ∗ ⌜ cur_even _ st__e = N ⌝ ∗ ⌜ cur_odd _ st__o = N ⌝ ∗ 
+      l ↦ #N ∗
       if Nat.even N
       then auth_even_at N ∗ auth_odd_at (N+1)
       else auth_even_at (N+1) ∗ auth_odd_at N.
   Definition evenodd_inv n := inv Ns (evenodd_inv_inner n).
 
-  Definition eo_corr n (N: nat) (γ: gname) (d: nat): iProp Σ :=
-    frag_model_is (N, N) ∗ n ↦ #N ∗
-    own γ (●E (if Nat.even (N + d) then N else (N + 1))).
-    
-  Definition eo_vs n ι γ d: iProp Σ :=
-    □ |={⊤, ⊤ ∖ ↑ι}=> ∃ (N: nat),
-    (▷ eo_corr n N γ d) ∗
-    (▷ (eo_corr n (if (Nat.even (N + d)) then (N + 1) else N) γ d) ={⊤ ∖ ↑ι, ⊤}=∗ True).
 
-  (* TODO: move *)
-  Lemma even_succ_negb n: Nat.even (S n) = negb $ Nat.even n.
-  Proof. by rewrite Nat.even_succ Nat.negb_even. Qed.
+  Let even_AM := @even_AM even_impl. 
+  Let odd_AM := @odd_AM odd_impl. 
 
-  (* TODO: move *)
-  Lemma odd_succ_negb n: Nat.odd (S n) = negb $ Nat.odd n.
-  Proof. by rewrite Nat.odd_succ Nat.negb_odd. Qed.
+  Definition st2nat (st: fmstate the_fair_model) N :=
+    cur_even even_impl st.1 = N /\ cur_odd odd_impl st.2 = N.
 
-  Lemma TMP_live_roles_same n m:
-    live_roles the_fair_model (n, n) = live_roles the_fair_model (m, m).
-  Proof. Admitted. 
-
-  Lemma eo_go_spec  (tid: locale heap_lang) n ρ (N: nat) f (Hf: f > 40) ι γ d
-    (STEP: forall k,
-        let k' := if (Nat.even (k + d)) then (k + 1) else k in
-        fmtrans the_fair_model (k, k) (Some ρ) (k', k'))
-        :
-    {{{  eo_vs n ι γ d ∗
-         has_fuels tid {[ ρ := f ]} ∗ own γ (◯E N) ∗
-         frag_free_roles_are ∅
-    }}}
-      incr_loop #n #N @ tid
-    {{{ RET #(); has_fuels tid ∅ }}}.
+  Lemma prod_AM_live_roles st__e st__o n
+    (CUR: st2nat (st__e, st__o) n)
+    :
+    AM_live_roles (@prod_AM_strong_lr even_impl odd_impl) (st__e, st__o) = 
+    set_map inl (AM_live_roles ame_strong st__e) ∪ set_map inr (AM_live_roles ame_strong st__o).
   Proof.
-    iLöb as "Hg" forall (N f Hf).
-    iIntros (Φ). iIntros "(#VS & Hf & Heven & HFR) Hk".
-
-    rewrite /incr_loop.
-    wp_lam.
-    wp_pures. wp_bind (CmpXchg _ _ _). iApply wp_atomic.
-    iPoseProof "VS" as "-#V". iMod "V" as "(%M & (>Hmod & >Hn & >Hauths) & CLOS)".
-
-    destruct (Nat.even (M + d)) eqn:Heqn.
-    - iDestruct (they_agree with "Heven Hauths") as "->".
-      iModIntro.
-      iApply (wp_step_model_singlerole with "Hmod Hf").
-      { specialize (STEP N). rewrite Heqn in STEP. apply STEP. }
-      {
-        (* TODO: derive from (abstracted) properties of submodels *)
-        erewrite TMP_live_roles_same. reflexivity. }
-      iApply (wp_cmpxchg_suc with "Hn"); [by do 3 f_equiv|done|].
-      iIntros "!> Hb Hmod Hf".
-      iMod (they_update _ _ _ (N + 2) with "[$]") as "[Hay Heven]".
-      wp_pures.
-      iModIntro.
-      iMod ("CLOS" with "[Hmod Hay Hb]") as "_". 
-      { iFrame. rewrite Nat.add_shuffle0.
-        rewrite (Nat.add_1_r (N + d)). 
-        subst.
-        rewrite even_succ_negb Heqn. simpl.
-        rewrite -Nat.add_assoc.
-        rewrite Nat2Z.inj_add. iFrame. }
-      iModIntro. simpl.
-
-      (* wp_pures. *) (*???*)
-      do 3 wp_pure _.
-      replace (Z.of_nat N + 2)%Z with (Z.of_nat (N + 2)) by lia.
-      iApply ("Hg" with "[] [Heven Hf HFR] [$]"); last first.
-      { iFrame "∗#". }
-      iPureIntro; lia.
-    - iDestruct (they_agree with "Heven Hauths") as "%Heq". rewrite -> Heq in *.
-      iModIntro.
-      subst. 
-      iApply (wp_step_model_singlerole with "Hmod Hf").
-      { specialize (STEP M). rewrite Heqn in STEP. apply STEP. }
-      { set_solver. }
-      iApply (wp_cmpxchg_fail with "Hn"); [intros Hne; simplify_eq; lia|done|].
-      iIntros "!> Hb Hmod Hf".
-      wp_pures.
-      iModIntro. 
-      iMod ("CLOS" with "[Hmod Hb Hauths]").
-      { iFrame.
-        by rewrite Heqn. }  
-      iModIntro. simpl.
-      (* wp_pures. *)
-      do 2 wp_pure _. 
-      iApply ("Hg" with "[] [Heven Hf HFR] [$]"); last first.
-      { iFrame "∗#". }
-      iPureIntro; lia.
-  Qed.
-
-  Lemma even_go_spec tid n (N: nat) f (Hf: f > 40) ι:
-    {{{  eo_vs n ι even_name 0 ∗
-         tid ↦M {[ inl ρT := f ]} ∗ own even_name (◯E N) ∗
-         frag_free_roles_are ∅
-    }}}
-      incr_loop #n #N @ tid
-    {{{ RET #(); tid ↦M ∅ }}}.
-  Proof.
-    apply eo_go_spec; auto.
-
-    (* !!! relies on transparent thread_model *)
-    intros k. rewrite Nat.even_add. rewrite Nat.add_1_r.  
-    destruct (Nat.even k) eqn:E. 
-    - simpl. eapply amfm_role_step with (a := inl (step_sync k)).
-      econstructor; eauto.
-      + econstructor. by rewrite Nat.even_add E.
-      + econstructor. rewrite Nat.add_1_r Nat.odd_succ. by rewrite E.
-    - simpl. eapply amfm_role_step with (a := inr (inl ())).
-      econstructor; eauto.
-      econstructor. rewrite Nat.add_0_r -Nat.negb_even E. done.
+    apply set_eq. intros ρ.
+    rewrite elem_of_union !elem_of_map.
+    setoid_rewrite <- AM_live_roles_spec.
+    destruct CUR as [CUR__e CUR__o]. simpl in *. 
+    split.
+    { intros (a & st' & STEP). inversion STEP; subst.
+      all: set_solver. } 
+    intros [(ρ__e & -> & (a__e & st__e' & STEP__e))| (ρ__o & -> & (a__o & st__o' & STEP__o))].
+    - destruct a__e as [[k] | a__e].
+      2: { eexists _, (_, _). eapply @pt_inner1; eauto.
+           Unshelve. 2: exact (inr $ inl a__e). done. }
+      forward eapply even_step_inv; eauto.
+      { apply STEP__e. }
+      intros (X & CUR__e' & E). assert (n = k) as -> by congruence. clear X. 
+      forward eapply odd_syncable; eauto.
+      { erewrite @f_equal; [apply E| ]. by f_equal. }
+      intros [st__o' STEP__o]. 
+      eexists _, (_, _). eapply @pt_sync1; eauto.  
+      Unshelve. 2: exact (inl $ step_sync k). simpl. congruence. 
+    - destruct a__o as [[k] | a__o].
+      2: { eexists _, (_, _). eapply @pt_inner2; eauto.
+           Unshelve. 2: exact (inr $ inr a__o). done. }
+      forward eapply odd_step_inv; eauto.
+      { apply STEP__o. }
+      intros (X & CUR__o' & O). assert (n = k) as -> by congruence. clear X. 
+      forward eapply even_syncable; eauto.
+      { erewrite @f_equal; [apply O| ]. by f_equal. }
+      intros [st__e' STEP__e]. 
+      eexists _, (_, _). eapply @pt_sync2; eauto.  
+      Unshelve. 2: exact (inl $ step_sync k). simpl. congruence. 
   Qed. 
 
-  Lemma odd_go_spec tid n (N: nat) f (Hf: f > 40) ι:
-    {{{  eo_vs n ι odd_name 1 ∗
-         tid ↦M {[ inr ρT := f ]} ∗ odd_at N ∗
-         frag_free_roles_are ∅
-    }}}
-      incr_loop #n #N @ tid
+  Lemma st2nat_step_ex st st' a oρ n
+    (STEP: amTrans prod_model st (a, oρ) st')
+    (CUR: st2nat st n):
+    exists n', st2nat st' n'.
+  Proof.
+    destruct st as [st__e st__o], st' as [st__e' st__o'].
+    destruct CUR as [CUR__e CUR__o]. simpl in *.
+    inversion STEP; subst.
+    - destruct a1.
+      { by destruct a as [|[|]]. }
+      destruct a; try done. 
+      eapply even_stutter_inv in STEP1. 
+      eexists. split; simpl. 
+      + by rewrite -STEP1.
+      + congruence.
+    - destruct a2.
+      { by destruct a as [|[|]]. }
+      destruct a; try done. 
+      eapply odd_stutter_inv in STEP2. 
+      eexists. split; simpl; 
+        revgoals. 
+      + by rewrite -STEP2.
+      + congruence.
+    - destruct a1 as [[]|], a2 as [[]|]; try by destruct a as [|[|]].
+      eapply even_step_inv in STEP1.
+      eapply odd_sync_inv in STEP2.
+      eexists. split; simpl. 
+      + apply STEP1. 
+      + lia.
+    - destruct a1 as [[]|], a2 as [[]|]; try by destruct a as [|[|]].
+      eapply even_sync_inv in STEP1.
+      eapply odd_step_inv in STEP2.
+      eexists. split; simpl;
+        revgoals. 
+      + apply STEP2. 
+      + lia.
+  Qed. 
+    
+
+  Lemma prod_step_lr_nonincr st st' a oρ n
+    (STEP: amTrans prod_model st (a, oρ) st')
+    (CUR: st2nat st n):
+      AM_live_roles prod_AM_strong_lr st' ⊆ AM_live_roles prod_AM_strong_lr st.
+  Proof.
+    destruct st as [st__e st__o], st' as [st__e' st__o'].
+    forward eapply st2nat_step_ex as [n' CUR']; eauto. 
+    erewrite !prod_AM_live_roles; eauto.
+    apply union_subseteq. eapply Morphisms_Prop.and_impl_morphism.
+    { red. eapply impl_transitive; [| apply union_subseteq_l'].
+      by apply set_map_mono. } 
+    { red. eapply impl_transitive; [| apply union_subseteq_r'].
+      by apply set_map_mono. }
+    inversion STEP; subst.
+    all: (try apply even_step_lr_nonincr in STEP1);
+      (try apply odd_step_lr_nonincr in STEP2); set_solver.
+  Qed. 
+
+  Let ρEven: fmrole M := inl (ρ__e even_impl).
+  Let ρOdd: fmrole M := inr (ρ__o odd_impl).
+
+  Lemma even_spec_use tid l (N : nat) f (Hf: f > 40) (ep: EvenProg):
+    {{{ evenodd_inv l ∗ tid ↦M {[ ρEven := f ]} ∗ even_at N }}}
+      (e_prog ep) #l #N @ tid
     {{{ RET #(); tid ↦M ∅ }}}.
   Proof.
-    apply eo_go_spec; auto.
-
-    (* !!! relies on transparent thread_model *)
-    intros k. rewrite Nat.add_1_r Nat.even_succ. 
-    destruct (Nat.odd k) eqn:O. 
-    - simpl. eapply amfm_role_step with (a := inl (step_sync k)).
-      econstructor; eauto.
-      + econstructor. by rewrite Nat.odd_add O.
-      + econstructor. rewrite Nat.add_1_r Nat.even_succ. by rewrite O.
-    - simpl. eapply amfm_role_step with (a := inr (inr ())).
-      econstructor; eauto.
-      econstructor. rewrite Nat.add_1_r odd_succ_negb O. done.
-  Qed.
-
-  (* TODO: move *)
-  Lemma if_sep_comm (b: bool) (P1 Q1 P2 Q2: iProp Σ):
-     (if b then (P1 ∗ Q1) else (P2 ∗ Q2)) ⊣⊢ (if b then P1 else P2) ∗ (if b then Q1 else Q2).
-  Proof. destruct b; set_solver. Qed. 
-
-  Lemma if_arg_comm {A B: Type} (b: bool) (x y: A) (f: A -> B):
-    (if b then f x else f y) = f (if b then x else y).
-  Proof. by destruct b. Qed. 
-
-  Inductive EO' := eoE | eoO.
+    iIntros (Φ) "(#Hinv & Hf & Heo) Hk".
+    
+    iApply (@e_spec ep the_fair_model _ _ _ evenThreadG 
+             with "[$Hf $Heo]"); [lia| simpl; lia | |done].
+    rewrite /eo_vs. iModIntro.
+    iMod (inv_acc with "Hinv") as "[OPEN CLOS]".
+    { apply top_subseteq. }
   
-  Definition eo_frag (eo: EO') : nat → iProp Σ :=
-    match eo with
-    | eoE => even_at
-    | eoO => odd_at
-    end.
+    iDestruct "OPEN" as (st__e st__o m) "(>Hmod & >%CUR__E & >%CUR__O & >Hn & Hauths)".
+    rewrite if_arg2_comm. iDestruct "Hauths" as "[E O]".
+    iModIntro. iExists _. iSplitL "Hn E".
+    { rewrite /eo_corr. simpl. iFrame.
+      simpl. iFrame. destruct (Nat.even m); auto. }
+    simpl.
 
-  (* !!! depends on known role of thread_model *)
-  Definition eo_role (eo: EO'): fmrole the_fair_model :=
-    match eo with
-    | eoE => inl ρT
-    | eoO => inr ρT
-    end.
+    iIntros (f') "MAP".
 
-  Lemma incr_loop_spec (eo : EO') tid n (N : nat) f (Hf: f > 40) :
-    {{{ evenodd_inv n ∗ tid ↦M {[ eo_role eo := f ]} ∗ (eo_frag eo) N ∗
-        frag_free_roles_are ∅ }}}
-      incr_loop #n #N @ tid
+    enough (exists st', fmtrans the_fair_model (st__e, st__o) (Some ρEven) st' /\
+                   st2nat st' (if Nat.even m then (m + 1) else m)) as (st' & TRANS & CUR'). 
+    { 
+
+      iApply (MU_wand with "[O CLOS]").
+      2: { iApply (model_step_MU with "[$] [MAP]"); eauto.
+           2: { eapply am_fmtrans_action in TRANS as (?&?). 
+                eapply prod_step_lr_nonincr; done. }
+           2: { iApply (has_fuels_proper with "[$]"); auto.
+                rewrite -(insert_empty _ f').
+                rewrite insert_union_singleton_l.
+                apply fin_maps.union_proper; [reflexivity| ].
+                by setoid_rewrite fmap_empty. }
+           done. }
+      iIntros "(MAP & ST)".
+      rewrite -insert_union_singleton_l.
+      iFrame. iSplitR; [iPureIntro; simpl; lia| ].
+      iIntros "(?&?)". iMod ("CLOS" with "[-]") as "_"; [| done].
+      rewrite /evenodd_inv_inner. iNext. iFrame.
+      destruct (Nat.even m) eqn:E.
+      - rewrite even_plus1_negb E. simpl. iFrame.
+        destruct st'. destruct CUR' as [??]. simpl in *. set_solver.
+      - rewrite E. destruct st'. iFrame.
+        destruct CUR' as [??]. simpl in *. set_solver. }
+ 
+    destruct (Nat.even m) eqn:E.
+    - forward eapply (even_steppable _ st__e) as (st__e' & STEP__e); eauto.
+      { set_solver. }
+      forward eapply odd_syncable as (st__o' & STEP__o); eauto.
+      { erewrite (f_equal Nat.even); eauto. }
+      rewrite CUR__E in STEP__e. rewrite CUR__O in STEP__o. 
+      eexists (_, _). split; [| split].
+      + simpl. econstructor. eapply @pt_sync1; eauto.
+        Unshelve. 2: exact (inl (step_sync m)). done. 
+      + simpl. eapply even_step_inv; eauto.
+      + simpl. eapply odd_sync_inv; eauto.
+    - pose proof E as O. rewrite -negb_true_iff Nat.negb_even in O. 
+      forward eapply (even_stutterable _ st__e) as (st__e' & a__e & STEP__e); eauto.
+      { rewrite CUR__E. intuition. }
+      eexists (_, _). split; [| split].
+      + simpl. econstructor. eapply @pt_inner1; eauto.
+        Unshelve. 2: exact (inr $ inl a__e). done.
+      + simpl. symmetry. rewrite -CUR__E. eapply even_stutter_inv; eauto.
+      + done. 
+  Qed.
+  
+  Lemma odd_spec_use tid l (N : nat) f (Hf: f > 40) (op: OddProg):
+    {{{ evenodd_inv l ∗ tid ↦M {[ ρOdd := f ]} ∗ odd_at N }}}
+      (o_prog op) #l #N @ tid
     {{{ RET #(); tid ↦M ∅ }}}.
   Proof.
-    iIntros (Φ) "(#Hinv & Hf & Heo & FR) Hk".
-    destruct eo; simpl in *. 
-    - iApply (even_go_spec with "[$Hf $FR $Heo]"); [lia| |done].
-      rewrite /eo_vs. iModIntro.
-      iMod (inv_acc with "Hinv") as "[OPEN CLOS]".
-      { apply top_subseteq. }
-      iDestruct "OPEN" as (M) "(>Hmod & >Hn & Hauths)".
-      rewrite if_sep_comm. iDestruct "Hauths" as "[E O]".      
-      iModIntro. iExists _. iSplitL "Hmod Hn E".
-      { iFrame. rewrite Nat.add_0_r. destruct (Nat.even M); auto. }
-      iIntros "(?&?&?)". iMod ("CLOS" with "[-]") as "_"; [| done].
-      iNext. iFrame.
-      rewrite !Nat.add_0_r.
-      rewrite if_sep_comm. destruct (Nat.even M) eqn:e.
-      + rewrite Nat.add_1_r. rewrite Nat.even_succ -Nat.negb_even.
-        rewrite e. simpl. iFrame. 
-      + rewrite e. iFrame.  
-    - iApply (odd_go_spec with "[$Hf $FR $Heo]"); [lia| |done].
-      rewrite /eo_vs. iModIntro.
-      iMod (inv_acc with "Hinv") as "[OPEN CLOS]".
-      { apply top_subseteq. }
-      iDestruct "OPEN" as (M) "(>Hmod & >Hn & Hauths)".
-      rewrite if_sep_comm. iDestruct "Hauths" as "[E O]".
-      iModIntro. iExists M.
-      rewrite /eo_corr. 
-      rewrite !(Nat.add_1_r M) Nat.even_succ.  
-      iSplitL "Hmod Hn O".
-      { iFrame. rewrite -Nat.negb_even. destruct (Nat.even M); simpl; auto. }
-      iIntros "(?&?&?)". iMod ("CLOS" with "[-]") as "_"; [| done].
-      iNext. iFrame.
-      rewrite if_sep_comm. destruct (Nat.odd M) eqn:e.
-      + rewrite Nat.add_1_r. rewrite !Nat.even_succ.
-        rewrite Nat.odd_succ -Nat.negb_odd.
-        rewrite e. iFrame.  
-      + rewrite Nat.add_1_r. rewrite !Nat.even_succ.
-        rewrite -Nat.negb_odd.
-        rewrite e. iFrame.  
+    iIntros (Φ) "(#Hinv & Hf & Heo) Hk".
+    
+    iApply (@o_spec op the_fair_model _ _ _ oddThreadG 
+             with "[$Hf $Heo]"); [lia| simpl; lia | |done].
+    rewrite /eo_vs. iModIntro.
+    iMod (inv_acc with "Hinv") as "[OPEN CLOS]".
+    { apply top_subseteq. }
+  
+    iDestruct "OPEN" as (st__e st__o m) "(>Hmod & >%CUR__E & >%CUR__O & >Hn & Hauths)".
+    rewrite if_arg2_comm. iDestruct "Hauths" as "[E O]".
+    iModIntro. iExists _. iSplitL "Hn O".
+    { rewrite /eo_corr. simpl. iFrame.
+      rewrite -Nat.negb_odd. destruct (Nat.odd m); iFrame. }
+    simpl.
+
+    iIntros (f') "MAP".
+
+    enough (exists st', fmtrans the_fair_model (st__e, st__o) (Some ρOdd) st' /\
+                   st2nat st' (if Nat.odd m then (m + 1) else m)) as (st' & TRANS & CUR'). 
+    { 
+
+      iApply (MU_wand with "[E CLOS]").
+      2: { iApply (model_step_MU with "[$] [MAP]"); eauto.
+           2: { eapply am_fmtrans_action in TRANS as (?&?). 
+                eapply prod_step_lr_nonincr; done. }
+           2: { iApply (has_fuels_proper with "[$]"); auto.
+                rewrite -(insert_empty _ f').
+                rewrite insert_union_singleton_l.
+                apply fin_maps.union_proper; [reflexivity| ].
+                by setoid_rewrite fmap_empty. }
+           done. }
+      iIntros "(MAP & ST)".
+      rewrite -insert_union_singleton_l.
+      iFrame. iSplitR; [iPureIntro; simpl; lia| ].
+      iIntros "(?&?)". iMod ("CLOS" with "[-]") as "_"; [| done].
+      rewrite /evenodd_inv_inner. iNext. iFrame.
+      rewrite -!Nat.negb_odd. 
+      destruct (Nat.odd m) eqn:O.
+      - simpl. rewrite !odd_plus1_negb O. simpl. iFrame.
+        destruct st'. destruct CUR' as [??]. simpl in *. set_solver.
+      - rewrite O. destruct st'. iFrame.
+        destruct CUR' as [??]. simpl in *. set_solver. }
+ 
+    destruct (Nat.odd m) eqn:O.
+    - forward eapply (odd_steppable _ st__o) as (st__o' & STEP__o); eauto.
+      { rewrite CUR__O. set_solver. }
+      forward eapply even_syncable as (st__e' & STEP__e); eauto.
+      { erewrite (f_equal Nat.odd); eauto. }
+      rewrite CUR__O in STEP__o. rewrite CUR__E in STEP__e. 
+      eexists (_, _). split; [| split].
+      + simpl. econstructor. eapply @pt_sync2; eauto.
+        Unshelve. 2: exact (inl (step_sync m)). done.
+      + simpl. eapply even_sync_inv; eauto.
+      + simpl. eapply odd_step_inv; eauto.
+    - pose proof O as E. rewrite -negb_true_iff Nat.negb_odd in E. 
+      forward eapply (odd_stutterable _ st__o) as (st__o' & a__o & STEP__o); eauto.
+      { rewrite CUR__O. intuition. }
+      eexists (_, _). split; [| split].
+      + simpl. econstructor. eapply @pt_inner2; eauto.
+        Unshelve. 2: exact (inr $ inr a__o). done.
+      + done. 
+      + simpl. symmetry. rewrite -CUR__O. eapply odd_stutter_inv; eauto.
   Qed.
 
 End proof.
 
 Section proof_start.
-  Context `{!heapGS Σ the_model, !evenoddG Σ}.
+  Context {even_impl: EvenModel} {odd_impl: OddModel}.
+  (* Let even_impl := thread_0_even.  *)
+  (* Let odd_impl := thread_1_odd. *)
+  Let M := @the_fair_model even_impl odd_impl.
+  Let LM := @the_model even_impl odd_impl.
+
+  Context (ep: EvenProg) (op: OddProg). 
+
+  Context `{!heapGS Σ LM, !evenoddG Σ}.
+  Context {th_preG: threadPreG Σ}. 
   Let Ns := nroot .@ "even_odd".
 
+  (* TODO: move *)
   Lemma frag_free_roles_are_sep: forall fr1 fr2 (DISJ: fr1 ## fr2), 
         frag_free_roles_are (fr1 ∪ fr2) ⊣⊢ frag_free_roles_are fr1 ∗ frag_free_roles_are fr2.
   Proof.
@@ -462,81 +380,82 @@ Section proof_start.
     rewrite -own_op. by rewrite -auth_frag_op.
   Qed. 
 
-  Let ρEven: fmrole the_fair_model := inl ρT.
-  Let ρOdd: fmrole the_fair_model := inr ρT.
+  Let ρEven: fmrole M := inl (ρ__e even_impl).
+  Let ρOdd: fmrole M := inr (ρ__o odd_impl).
 
-  Lemma start_spec tid n N1 N2 f (Hf: f > 60) :
-    {{{ evenodd_inv n ∗ tid ↦M {[ inl ρT := f; inr ρT := f ]} ∗
+  Definition start : val :=
+    λ: "l",
+      let: "x" := !"l" in
+      (Fork ((e_prog ep) "l" "x") ;;
+       Fork ((o_prog op) "l" ("x"+#1))).
+
+  Existing Instance even_AME. 
+  Existing Instance odd_AME.
+
+  Lemma start_spec tid n N1 N2 f (Hf: f > 60) (EVEN: N1 < N2)
+    :
+    {{{ evenodd_inv n ∗ 
+        tid ↦M {[ ρEven := f; ρOdd := f ]} ∗
         even_at N1 ∗ odd_at N2 ∗ frag_free_roles_are ∅ }}}
       start #n @ tid
     {{{ RET #(); tid ↦M ∅ }}}.
   Proof using All.
     iIntros (Φ) "(#Hinv & Hf & Heven_at & Hodd_at & HFR) HΦ". unfold start.
     rewrite <- (union_empty_l_L ∅). 
-    iDestruct (frag_free_roles_are_sep with "HFR") as "[HFR1 HFR2]"; [set_solver| ].
+    (* iDestruct (frag_free_roles_are_sep with "HFR") as "[HFR1 HFR2]"; [set_solver| ]. *)
     wp_pures.
     wp_bind (Load _).
     iApply wp_atomic.
-    iInv Ns as (M) "(>Hmod & >Hn & Hauths)" "Hclose".
+    iInv Ns as (st__e st__o m) "(>Hmod & >%CUR__E & >%CUR__O & >Hn & Hauths)" "Hclose".
     iIntros "!>". wp_load. iIntros "!>".
     
-    rewrite if_sep_comm !if_arg_comm.
+    rewrite if_arg2_comm !if_arg_comm.
     iDestruct "Hauths" as "[Heven Hodd]".
-    iDestruct (even_agree with "Heven_at Heven") as %<-.
-    iDestruct (odd_agree with "Hodd_at Hodd") as %<-.
+    iDestruct (th_agree with "Heven_at Heven") as %<-.
+    iDestruct (th_agree with "Hodd_at Hodd") as %<-.
+    destruct (Nat.even m) eqn:E; [| lia].
 
-    iAssert ((if Nat.even M then auth_even_at else auth_odd_at) M ∗
-             (if Nat.even M then auth_odd_at else auth_even_at) (M + 1))%I
-      with "[Heven Hodd] "as "[CUR_AUTH NEXT_AUTH]".
-    { destruct (Nat.even M); iFrame. }
-
-    iAssert ((if Nat.even M then even_at else odd_at) M ∗
-             (if Nat.even M then odd_at else even_at) (M + 1))%I
-      with "[Heven_at Hodd_at] "as "[CUR NEXT]".
-    { destruct (Nat.even M); iFrame. }
-
-    iMod ("Hclose" with "[-Hf CUR NEXT HΦ HFR1 HFR2]") as "_".
-    { iIntros "!>". iExists _. iFrame.
-      destruct (Nat.even M); iFrame. }
+    iMod ("Hclose" with "[-Hf Heven_at Hodd_at HΦ]") as "_".
+    { iIntros "!>". iExists _. iFrame. 
+      rewrite E. iFrame; done. }
     iIntros "!>". wp_pures. wp_bind (Fork _).
-    iApply (wp_role_fork _ tid _ _ _ {[if Nat.even M then ρOdd else ρEven := _]}
-                         {[if Nat.even M then ρEven else ρOdd := _]}
-             with "[Hf ] [CUR HFR1]"). 
+    iApply (wp_role_fork _ tid _ _ _ {[ρOdd := _]} {[ρEven := _]}
+             with "[Hf ] [Heven_at]"). 
     { apply map_disjoint_dom. rewrite !dom_singleton.
-      destruct (Nat.even M); set_solver. }
+      destruct (Nat.even m); set_solver. }
     { intros Hempty%map_positive_l. set_solver. }
     { rewrite has_fuels_gt_1; last solve_fuel_positive.
-      rewrite !fmap_insert fmap_empty //.      
+      rewrite !fmap_insert fmap_empty //.
       iApply has_fuels_proper; [..| by iFrame]; auto.
       rewrite !insert_union_singleton_l map_union_empty.
-      destruct (Nat.even M); try reflexivity.
-      f_equiv. rewrite map_union_comm; auto. apply map_disjoint_dom. set_solver. }
+      rewrite map_union_comm; [reflexivity| ].
+      rewrite map_disjoint_dom. set_solver. }
     { iIntros (tid') "!> Hf".
-      iApply (incr_loop_spec (if Nat.even M then eoE else eoO) with "[-]").
-      2: { destruct (Nat.even M); iFrame "#∗". }
+      iApply (even_spec_use with "[-]").
+      2: { iFrame "#∗". }
       { lia. }
       intuition. }
 
     iIntros "!> Hf".
     iIntros "!>".
     wp_pures.
-    iApply (wp_role_fork _ tid _ _ _ ∅ _ with "[Hf] [NEXT HFR2]").
+    iApply (wp_role_fork _ tid _ _ _ ∅ _ with "[Hf] [Hodd_at]").
     { apply map_disjoint_dom. apply map_disjoint_dom. apply map_disjoint_empty_l. }
     2: { rewrite has_fuels_gt_1; last solve_fuel_positive.
          rewrite !fmap_insert fmap_empty //.
          rewrite insert_union_singleton_l. 
          rewrite map_union_comm; [done|].
          apply map_disjoint_dom. set_solver. }
-    { rewrite map_empty_union. destruct (Nat.even M); set_solver. }
+    { rewrite map_empty_union. set_solver. }
     { iIntros (tid') "!> Hf".
       wp_pures.
-      replace (Z.of_nat M + 1)%Z with (Z.of_nat (M + 1)) by lia.
-      iApply (incr_loop_spec (if Nat.even M then eoO else eoE) with "[-]").
-      2: { destruct (Nat.even M); iFrame "#∗". }
+      replace (Z.of_nat m + 1)%Z with (Z.of_nat (m + 1)) by lia.
+      iApply (odd_spec_use with "[-]").
+      2: { iFrame "#∗". }
       { lia. }
       intuition. }
 
     iIntros "!> Hf". by iApply "HΦ".
-  Qed.
+  Qed. 
 
 End proof_start.
